theories/Lambda.v
@@ -4,27 +4,27 @@ Require Import Coq.Relations.Relation_Definitions.
 (* The ordinary λ-calculus *)
 (* ----------------------- *)
 
-Inductive λ: Type :=
+Inductive term: Type :=
 | Var (x: var)
-| Lam (t: {bind λ})
-| App (s t: λ).
+| Lam (t: {bind term})
+| App (s t: term).
 
 (* autosubst sorcery *)
 (* ----------------- *)
 
-Instance Ids_λ : Ids λ. derive. Defined.
-Instance Rename_λ : Rename λ. derive. Defined.
-Instance Subst_λ : Subst λ. derive. Defined.
-Instance SubstLemmas_λ : SubstLemmas λ. derive. Defined.
+Instance Ids_term : Ids term. derive. Defined.
+Instance Rename_term : Rename term. derive. Defined.
+Instance Subst_term : Subst term. derive. Defined.
+Instance SubstLemmas_term : SubstLemmas term. derive. Defined.
 
 (* beta reduction *)
 (* -------------- *) 
 
-Inductive step : relation λ :=
+Inductive step : relation term :=
 | Step_Beta s s' t : s' = s.[t .: ids] ->
                      step (App (Lam s) t) s'
-| Step_Abs s s' : step s s' ->
-                  step (Lam s) (Lam s')
+| Step_Abs (s s': {bind term}) : step s s' ->
+                                 step (Lam s) (Lam s')
 | Step_App1 s s' t: step s s' ->
                     step (App s t) (App s' t)
 | Step_App2 s t t': step t t' ->
@@ -35,12 +35,16 @@ Inductive step : relation λ :=
 
 Require Import SimpleTypes.
 
-Inductive sequent (Γ: var->type) : λ -> type -> Prop := 
+Inductive sequent (Γ: var->type) : term -> type -> Prop := 
 | Ax (x: var) (A: type) :
-  Γ x = A -> sequent Γ (Var x) A
+  Γ x = A ->
+  sequent Γ (Var x) A
 
-| Intro (t: λ) (A B: type) :
-  sequent (A .: Γ) t B -> sequent Γ (Lam t) (Arr A B)
+| Intro (t: term) (A B: type) :
+  sequent (A .: Γ) t B ->
+  sequent Γ (Lam t) (Arr A B)
                                  
-| Elim (s t: λ) (A B: type) :
-  sequent Γ s (Arr A B) -> sequent Γ t A -> sequent Γ (App s t) B.
+| Elim (s t: term) (A B: type) :
+  sequent Γ s (Arr A B) ->
+  sequent Γ t A ->
+  sequent Γ (App s t) B.
